LocaleLTS.thy
@@ -4,51 +4,51 @@ imports Main
 
 begin
 
-section {* Labelled transition systems *}
+section {* Labeled transition systems *}
 
 text {* The semantics of a B component is a discrete, eventful, state-transition systems. We 
-first define what is meant exactly by such systems. Any system is, at a given time in a state. 
-Conversely, a system has a set of possible states. A system evolves from state to state,
-and such changes called transitions. Also when a system makes a transition, this is observable
-and this observation is called an event. State, transition and event are three different
-entities and a type is declared for each: *}
+formalize such systems. First, the notion of labeled \emph{transition} is specified. A transition
+has source and destination state, and is labeled by an event. The type for states and events
+is left abstract for now, and we thus define a parametric record type:*}
 
-locale Transition =
-fixes 
-  src :: "'trans \<Rightarrow> 'state" and
-  dst :: "'trans \<Rightarrow> 'state" and
-  evt :: "'trans \<Rightarrow> 'event"
+record ('st, 'ev) Transition =
+  src :: 'st
+  dst :: 'st
+  lbl :: 'ev
+
+text {* Next we specify a \emph{labeled transition system}. Such system is fully defined
+by a set of initial states, and a set of transitions: *}
+
+record ('st, 'ev) LTS =
+  init :: "'st set"
+  trans :: "('st, 'ev) Transition set"
   
-locale LTS = Transition src dst evt 
-for
-  src :: "'trans \<Rightarrow> 'state" and
-  dst :: "'trans \<Rightarrow> 'state" and
-  evt :: "'trans \<Rightarrow> 'event"
-+
+locale LTS =
 fixes
-  init :: "'state set" and
-  trans :: "'trans set"
+  lts :: "('st, 'ev) LTS"
 begin
 
-  inductive_set states :: "'state set" where
-      base[elim!]: "s \<in> init \<Longrightarrow> s \<in> states"
-    | step[elim!]: "\<lbrakk> t \<in> trans; src t \<in> states \<rbrakk> \<Longrightarrow> dst t \<in> states"
+text {* The (reachable) \emph{states} of a LTS are defined inductively, as follows. *}
 
-  definition successors :: "'state set \<Rightarrow> 'state set" where
-    "successors S \<equiv> { s | s . \<exists> t \<in> trans . src t \<in> S \<and> dst t = s}"
+  inductive_set states :: "'st set" where
+      base[elim!]: "s \<in> init lts \<Longrightarrow> s \<in> states"
+    | step[elim!]: "\<lbrakk> t \<in> trans lts; src t \<in> states \<rbrakk> \<Longrightarrow> dst t \<in> states"
+
+  definition successors :: "'st set \<Rightarrow> 'st set" where
+    "successors S \<equiv> { s | s . \<exists> t \<in> trans lts . src t \<in> S \<and> dst t = s}"
   
-  lemma reachable_init: "init \<subseteq> states" by auto
+  lemma reachable_init: "init lts \<subseteq> states" by auto
 
   lemma reachable_stable: "successors states \<subseteq> states"
     unfolding successors_def by auto
 
-text {* The following lemma is related to the identification of sufficient conditions to establish 
+text {* The following lemma is useful to identify sufficient conditions to establish 
 safety properties. Consider a property that is satisfied by some set of states $S$. If the initial 
 states are in $S$, and if the successors of $S$ are in $S$ then all the reachable states are in 
-$S$. *}
+$S$: *}
 
   lemma reachable_induct_set:
-    assumes base: "init \<subseteq> S" and step: "successors S \<subseteq> S"
+    assumes base: "init lts \<subseteq> S" and step: "successors S \<subseteq> S"
     shows "states \<subseteq> S"
   proof
     fix x
@@ -56,11 +56,11 @@ $S$. *}
     thus "x \<in> S"
     proof (induct x)
       fix i
-      assume "i \<in> init"
+      assume "i \<in> init lts"
       with base show "i \<in> S" ..
     next
       fix t
-      assume "t \<in> trans" "src t \<in> states" "src t \<in> S"
+      assume "t \<in> trans lts" "src t \<in> states" "src t \<in> S"
       with step show "dst t \<in> S" unfolding successors_def by auto
     qed
   qed
@@ -68,8 +68,8 @@ $S$. *}
 text {* Next we enunciate and prove a similar lemma for predicates. *}
 
 lemma reachable_induct_predicate:
-  assumes base: "\<forall> s \<in> init . p s" and 
-          step: "\<forall> t \<in> trans . p (src t) \<longrightarrow> p (dst t)"
+  assumes base: "\<forall> s \<in> init lts . p s" and 
+          step: "\<forall> t \<in> trans lts . p (src t) \<longrightarrow> p (dst t)"
   shows "\<forall> s \<in> states . p s"
 proof
   fix x
@@ -77,14 +77,28 @@ proof
   thus "p x"
   proof (induct x)
     fix i
-    assume "i \<in> init"
+    assume "i \<in> init lts"
     with base show "p i" ..
   next
     fix t
-    assume "t \<in> trans" "src t \<in> states" "p (src t)"
+    assume "t \<in> trans lts" "src t \<in> states" "p (src t)"
     with step show "p (dst t)" unfolding successors_def by auto
   qed
 qed
+
+subsection {* Behavior *}
+
+text {* Internal behavior. *}
+
+  inductive_set runs :: "('st, 'ev) Transition list set" where
+      base: "[] : runs"
+    | one[elim!]: "\<lbrakk> t \<in> trans lts; src t \<in> init lts \<rbrakk> \<Longrightarrow> [t] \<in> runs"
+    | step[elim!]: "\<lbrakk> t \<in> trans lts; r \<in> runs; r \<noteq> []; src t = dst (last r) \<rbrakk> \<Longrightarrow> r @ [t] \<in> runs"
+
+text {* External behavior. *}
+
+  definition traces :: "'ev list set" where
+    "traces \<equiv> { map lbl r | r . r \<in> runs }"
 
 end
 
