Simulation.thy
@@ -10,113 +10,67 @@ and the states of another LTS such that any transition taken by the former can b
 by the latter, i.e. the latter can follow a transition that is labeled with the same event,
 and leads to a state where it can continue the simulation: *}
 
-definition lts_simulation_init :: "STATE rel \<Rightarrow> LTS \<Rightarrow> LTS \<Rightarrow> bool" where
-  "lts_simulation_init r l1 l2 \<equiv> \<forall> s1 \<in> init l1 . \<exists> s2 \<in> init l2 . (s1, s2) \<in> r"
+definition simulation_init :: "'st rel \<Rightarrow> ('st, 'ev) LTS \<Rightarrow> ('st, 'ev) LTS \<Rightarrow> bool" where
+  "simulation_init r l1 l2 \<equiv> \<forall> s1 \<in> init l1 . \<exists> s2 \<in> init l2 . (s1, s2) \<in> r"
 
-definition lts_simulation_transition :: "STATE rel \<Rightarrow> LTS \<Rightarrow> LTS \<Rightarrow> bool" where
-  "lts_simulation_transition r l1 l2 \<equiv> 
+definition simulation_step :: "'st rel \<Rightarrow> ('st, 'ev) LTS \<Rightarrow> ('st, 'ev) LTS \<Rightarrow> bool" where
+  "simulation_step r l1 l2 \<equiv> 
     \<forall> s1 s2 . (s1, s2) \<in> r \<longrightarrow>
       (\<forall> t1 \<in> trans l1 . src t1 = s1 \<longrightarrow>
-        (\<exists> t2 \<in> trans l2 . src t2 = s2 \<and> evt t1 = evt t2 \<and> (dst t1, dst t2) \<in> r))"
+        (\<exists> t2 \<in> trans l2 . src t2 = s2 \<and> lbl t1 = lbl t2 \<and> (dst t1, dst t2) \<in> r))"
 
-definition lts_simulation :: "STATE rel \<Rightarrow> LTS \<Rightarrow> LTS \<Rightarrow> bool" where
-  "lts_simulation r l1 l2 \<equiv> lts_simulation_init r l1 l2 \<and> lts_simulation_transition r l1 l2"
+definition simulation :: "'st rel \<Rightarrow> ('st, 'ev) LTS \<Rightarrow> ('st, 'ev) LTS \<Rightarrow> bool" where
+  "simulation r l1 l2 \<equiv> simulation_init r l1 l2 \<and> simulation_step r l1 l2"
 
 text {* Let us verify some basic properties of simulations. First we have that the
 identity relation establishes that a LTS simulates itself. *}
   (* maybe use Id_on (states l) instead of Id ? *)
-lemma lts_simulation_identity :
-  "lts_simulation Id l l" unfolding lts_simulation_def
-proof
-  show "lts_simulation_init Id l l" unfolding lts_simulation_init_def Id_def by auto
-next
-  show "lts_simulation_transition Id l l" unfolding lts_simulation_transition_def Id_def by auto
-qed
+lemma simulation_identity : "simulation Id l l" 
+  unfolding simulation_def simulation_init_def simulation_step_def by auto
 
 text {* Second, we have that the composition of two simulation relations 
 is a simulation relation. *}
-lemma lts_simulation_transitivity:
-assumes s12: "lts_simulation r12 l1 l2" and s23: "lts_simulation r23 l2 l3"
-shows "lts_simulation (r12 O r23) l1 l3"
+lemma simulation_transitivity:
+assumes s12: "simulation r12 l1 l2" and s23: "simulation r23 l2 l3"
+shows "simulation (r12 O r23) l1 l3"
 proof -
-  have "lts_simulation_init (r12 O r23) l1 l3"
-  proof -
-    from s12 have "lts_simulation_init r12 l1 l2" unfolding lts_simulation_def ..
-  moreover
-    from s23 have "lts_simulation_init r23 l2 l3" unfolding lts_simulation_def ..
-  ultimately
-    show "lts_simulation_init (r12 O r23) l1 l3" unfolding lts_simulation_init_def relcomp_def by blast
-  qed
+  from s12 s23
+  have "simulation_init (r12 O r23) l1 l3"
+  unfolding simulation_def simulation_init_def relcomp_unfold
+  by simp metis
 moreover
-  have "lts_simulation_transition (r12 O r23) l1 l3" unfolding "lts_simulation_transition_def"
-  proof
-    fix s1
-    show "\<forall>s3. (s1, s3) \<in> r12 O r23 \<longrightarrow> (\<forall>t1\<in>LTS.trans l1. src t1 = s1 \<longrightarrow> (\<exists>t2\<in>LTS.trans l3. src t2 = s3 \<and> evt t1 = evt t2 \<and> (dst t1, dst t2) \<in> r12 O r23))"
-    proof
-      fix s3
-      show "(s1, s3) \<in> r12 O r23 \<longrightarrow> (\<forall>t1\<in>LTS.trans l1. src t1 = s1 \<longrightarrow> (\<exists>t2\<in>LTS.trans l3. src t2 = s3 \<and> evt t1 = evt t2 \<and> (dst t1, dst t2) \<in> r12 O r23))"
-      proof
-        assume 1: "(s1, s3) \<in> r12 O r23"
-        show "(\<forall>t1\<in>LTS.trans l1. src t1 = s1 \<longrightarrow> (\<exists>t2\<in>LTS.trans l3. src t2 = s3 \<and> evt t1 = evt t2 \<and> (dst t1, dst t2) \<in> r12 O r23))"
-        proof
-          fix t1
-          assume dom_t1: "t1\<in>LTS.trans l1"
-          show "src t1 = s1 \<longrightarrow> (\<exists>t3\<in>LTS.trans l3. src t3 = s3 \<and> evt t1 = evt t3 \<and> (dst t1, dst t3) \<in> r12 O r23)"
-          proof
-            assume src_t1: "src t1 = s1"
-            show "\<exists>t3\<in>LTS.trans l3. src t3 = s3 \<and> evt t1 = evt t3 \<and> (dst t1, dst t3) \<in> r12 O r23"
-              proof-
-                have "\<exists> t3 . t3 \<in> LTS.trans l3 \<and> src t3 = s3 \<and> evt t1 = evt t3 \<and> (dst t1, dst t3) \<in> r12 O r23"
-                proof -
-                  from 1 have "\<exists> s2 . (s1, s2) \<in> r12 \<and> (s2, s3) \<in> r23" unfolding relcomp_def by auto
-                  then obtain s2 where 2: "(s1, s2) \<in> r12 \<and> (s2, s3) \<in> r23" ..
-                moreover
-                  from 2 have "(s1, s2) \<in> r12" ..
-                  with s12 src_t1 dom_t1 obtain t2 where w12: "t2 \<in> LTS.trans l2 \<and> src t2 = s2 \<and> evt t1 = evt t2 \<and> (dst t1, dst t2) \<in> r12" 
-                    unfolding lts_simulation_def lts_simulation_transition_def by blast
-                moreover
-                  from 2 have "(s2, s3) \<in> r23" by simp
-                  with s23 w12 obtain w where "w \<in> LTS.trans l3 \<and> src w = s3 \<and> evt t2 = evt w \<and> (dst t2, dst w) \<in> r23" 
-                    unfolding lts_simulation_def lts_simulation_transition_def by blast
-                  with w12 have "w \<in> LTS.trans l3 \<and> src w = s3 \<and> evt t1 = evt w \<and> (dst t1, dst w) \<in> r12 O r23" unfolding relcomp_def by auto
-                  then show ?thesis ..
-                qed
-              then show ?thesis by auto
-            qed
-          qed
-        qed
-      qed
-    qed
-  qed
-  ultimately show ?thesis unfolding lts_simulation_def ..
+  from s12 s23
+  have "simulation_step (r12 O r23) l1 l3"
+  unfolding simulation_step_def simulation_def relcomp_unfold
+  by simp metis
+  ultimately show ?thesis unfolding simulation_def ..
 qed
 
 text {* Next we carry these properties over to the simulates relation over LTS. *}
 
 text {* Based on the notion of simulation, we introduce the relation simulates on LTS: *}
-definition lts_simulates :: "LTS \<Rightarrow> LTS \<Rightarrow> bool" (infixl "\<sim>" 50) where
-  "(l1 \<sim> l2) \<equiv> \<exists> r . lts_simulation r l2 l1"
+definition simulates :: "('st, 'ev) LTS \<Rightarrow> ('st, 'ev) LTS \<Rightarrow> bool" (infixl "\<sim>" 50) where
+  "(l1 \<sim> l2) \<equiv> \<exists> r . simulation r l2 l1"
 
-lemma lts_simulates_reflexivity: "l \<sim> l" 
-  unfolding lts_simulates_def
+lemma simulates_reflexivity: "l \<sim> l" 
+  unfolding simulates_def
 proof
-  show "lts_simulation Id l l" by (rule lts_simulation_identity)
+  show "simulation Id l l" by (rule simulation_identity)
 qed
 
-lemma lts_simulates_transitivity:
+lemma simulates_transitivity:
 assumes
   s12: "l1 \<sim> l2" and s23: "l2 \<sim> l3"
 shows
   "l1 \<sim> l3"
 proof -
-  from s23 obtain s where "lts_simulation s l3 l2" unfolding lts_simulates_def ..
+  from s23 obtain s where "simulation s l3 l2" unfolding simulates_def ..
 moreover
-  from s12 obtain r where "lts_simulation r l2 l1" unfolding lts_simulates_def ..
+  from s12 obtain r where "simulation r l2 l1" unfolding simulates_def ..
 ultimately
-  have "lts_simulation (s O r) l3 l1" 
-    by (rule lts_simulation_transitivity[of "s" "l3" "l2" "r" "l1"])
-  then have "\<exists> r . lts_simulation r l3 l1" ..
-  then show ?thesis unfolding lts_simulates_def by simp
+  have "simulation (s O r) l3 l1" 
+    by (rule simulation_transitivity[of "s" "l3" "l2" "r" "l1"])
+  then show ?thesis unfolding simulates_def by auto
 qed
   
 end
