LocaleMachine.thy
@@ -1,0 +1,27 @@
+theory LocaleMachine
+
+imports Main LocaleLTS
+
+begin
+
+locale Machine =
+  LTS lts
+for
+  lts :: "('state, 'event) LTS" 
++
+fixes
+  inv :: "'state \<Rightarrow> bool"
+begin
+
+  definition sound :: "bool" where
+    "sound \<equiv> \<forall> s \<in> states . (inv s)"
+  
+  lemma po:
+  assumes po_init: "\<forall> s \<in> init lts. inv s" and
+          po_step: "\<forall> t \<in> trans lts. inv (src t) \<longrightarrow> inv (dst t)"
+  shows sound
+  unfolding sound_def sorry 
+
+end
+
+end
