LocaleRefinement.thy
@@ -1,0 +1,22 @@
+theory LocaleRefinement
+
+imports Main LocaleLTS LocaleSimulation
+
+begin
+
+locale Refinement =
+  abstract: LTS la
++ concrete: LTS lc
+for
+  la :: "('astate, 'event) LTS" and
+  lc :: "('cstate, 'event) LTS"
++ 
+fixes 
+  inv :: "'astate \<times> 'cstate \<Rightarrow> bool"
+begin
+  definition sound :: bool where
+    "sound \<equiv> true"
+end
+
+
+end
