LocaleSimulation.thy
@@ -1,9 +1,7 @@
 theory LocaleSimulation
-
 imports Main LocaleLTS
-
 begin
-section {* Behaviour: a set of traces *}
+section {* Simulation *}
 
 text {* We introduce the notion of simulation: a relation between the states of one LTS
 and the states of another LTS such that any transition taken by the former can be simulated
@@ -11,131 +9,79 @@ by the latter, i.e. the latter can follow a transition that is labeled with the 
 and leads to a state where it can continue the simulation: *}
 
 locale Simulation =
-  abstract: LTS asrc adst aevt ainit atrans
-+ concrete: LTS csrc cdst cevt cinit ctrans
-for
-  asrc :: "'atrans \<Rightarrow> 'astate" and
-  adst :: "'atrans \<Rightarrow> 'astate" and
-  aevt :: "'atrans \<Rightarrow> 'event" and
-  ainit :: "'astate set" and
-  atrans :: "'atrans set" and
-  csrc :: "'ctrans \<Rightarrow> 'cstate" and
-  cdst :: "'ctrans \<Rightarrow> 'cstate" and
-  cevt :: "'ctrans \<Rightarrow> 'event" and
-  cinit :: "'cstate set" and
-  ctrans :: "'ctrans set"
-+
+  abstract: LTS la 
++ 
+  concrete: LTS lc
+for 
+  la :: "('a, 'ev) LTS" and  lc :: "('c, 'ev) LTS"
++ 
 fixes
-  r :: "('astate \<times> 'cstate) set"
+  r :: "('a \<times> 'c) set"
 assumes
-  rinit: "\<forall> cs \<in> cinit . \<exists> as \<in> ainit . (as, cs) \<in> r" and
-  rtrans: "\<forall> as cs . (as, cs) \<in> r \<longrightarrow> (\<forall> ct \<in> ctrans . csrc ct = cs \<longrightarrow>
-              (\<exists> at \<in> atrans . asrc at = as \<and> aevt at = cevt ct \<and> (adst at, cdst ct) \<in> r))"
+  rinit: "\<forall> cs \<in> init lc. \<exists> as \<in> init la. (as, cs) \<in> r" and
+  rtrans: "\<forall> as cs . (as, cs) \<in> r \<longrightarrow> (\<forall> ct \<in> trans lc. src ct = cs \<longrightarrow>
+              (\<exists> at \<in> trans la. src at = as \<and> lbl at = lbl ct \<and> (dst at, dst ct) \<in> r))"
 begin
 end
 
+text {* One simple property involving simulations is that the identity relation $Id$
+defines a simulation of an LTS $l$by itself. This is expressed and showed in a context
+containing the definition of LTS, as follows: *}
 sublocale LTS \<subseteq>
-          Simulation src dst evt init trans 
-                     src dst evt init trans
-                     Id
+          Simulation lts lts Id
 by unfold_locales auto
 
 locale SimulationComposition =
-  sim1: Simulation asrc adst aevt ainit atrans msrc mdst mevt minit mtrans r1
-+ sim2: Simulation msrc mdst mevt minit mtrans csrc cdst cevt cinit ctrans r2
+  sim1: Simulation la lb r1 + sim2: Simulation lb lc r2
 for
-  asrc :: "'atrans \<Rightarrow> 'astate" and
-  adst :: "'atrans \<Rightarrow> 'astate" and
-  aevt :: "'atrans \<Rightarrow> 'event" and
-  ainit :: "'astate set" and
-  atrans :: "'atrans set" and
-  msrc :: "'mtrans \<Rightarrow> 'mstate" and
-  mdst :: "'mtrans \<Rightarrow> 'mstate" and
-  mevt :: "'mtrans \<Rightarrow> 'event" and
-  minit :: "'mstate set" and
-  mtrans :: "'mtrans set" and
-  r1 :: "('astate \<times> 'mstate) set" and
-  csrc :: "'ctrans \<Rightarrow> 'cstate" and
-  cdst :: "'ctrans \<Rightarrow> 'cstate" and
-  cevt :: "'ctrans \<Rightarrow> 'event" and
-  cinit :: "'cstate set" and
-  ctrans :: "'ctrans set" and
-  r2 :: "('mstate \<times> 'cstate) set"
+  la :: "('a, 'ev) LTS" and lb :: "('b, 'ev) LTS" and lc :: "('c, 'ev) LTS" and
+  r1 :: "('a \<times> 'b) set" and r2 :: "('b \<times> 'c) set"
+begin
+end
 
 sublocale SimulationComposition \<subseteq> 
-          Simulation asrc adst aevt ainit atrans
-                     csrc cdst cevt cinit ctrans
-                     "r1 O r2"
+          Simulation la lc "r1 O r2"
 proof 
-  from sim1.rinit sim2.rinit show "\<forall> cs \<in> cinit. \<exists> as \<in> ainit. (as, cs) \<in> r1 O r2"
+  from sim1.rinit sim2.rinit show "\<forall> cs \<in> init lc. \<exists> as \<in> init la. (as, cs) \<in> r1 O r2"
     unfolding relcomp_unfold by simp metis
 next
   from sim1.rtrans sim2.rtrans 
   show "\<forall>as cs. (as, cs) \<in> r1 O r2 \<longrightarrow> 
-         (\<forall>ct\<in>ctrans. csrc ct = cs \<longrightarrow> 
-           (\<exists>at\<in>atrans. asrc at = as \<and> aevt at = cevt ct \<and> (adst at, cdst ct) \<in> r1 O r2))"
+         (\<forall> ct \<in> trans lc. src ct = cs \<longrightarrow> 
+           (\<exists> at \<in> trans la. src at = as \<and> lbl at = lbl ct \<and> (dst at, dst ct) \<in> r1 O r2))"
     unfolding relcomp_unfold by simp metis
 qed
 
-text {* Based on the notion of simulation, we introduce the relation simulates on LTS: *}
+text {* We introduce the relation simulates on LTS. Is there a way to use the locale Simulation
+in this definition? *}
 
 locale Simulate =
-  abstract: LTS asrc adst aevt ainit atrans
-+ concrete: LTS csrc cdst cevt cinit ctrans
-+ sim: Simulation asrc adst aevt ainit atrans csrc cdst cevt cinit ctrans r
+  abstract: LTS la + concrete: LTS lc
 for
-  asrc :: "'atrans \<Rightarrow> 'astate" and
-  adst :: "'atrans \<Rightarrow> 'astate" and
-  aevt :: "'atrans \<Rightarrow> 'event" and
-  ainit :: "'astate set" and
-  atrans :: "'atrans set" and
-  csrc :: "'ctrans \<Rightarrow> 'cstate" and
-  cdst :: "'ctrans \<Rightarrow> 'cstate" and
-  cevt :: "'ctrans \<Rightarrow> 'event" and
-  cinit :: "'cstate set" and
-  ctrans :: "'ctrans set" and
-  r :: "('astate \<times> 'cstate) set"
+  la :: "('a, 'ev) LTS" and lc :: "('c, 'ev) LTS"
++
+assumes
+  "\<exists> r . ((\<forall> cs \<in> init lc. \<exists> as \<in> init la. (as, cs) \<in> r) \<and>
+          (\<forall> as cs . (as, cs) \<in> r \<longrightarrow> (\<forall> ct \<in> trans lc. src ct = cs \<longrightarrow>
+              (\<exists> at \<in> trans la. src at = as \<and> lbl at = lbl ct \<and> (dst at, dst ct) \<in> r))))"
 begin
 end
 
-sublocale LTS \<subseteq> 
-          Simulate src dst evt init trans
-                   src dst evt init trans
-                   Id
+sublocale Simulation \<subseteq> Simulate la lc
+sorry
+  
+sublocale LTS \<subseteq> Simulate l l
 by unfold_locales auto
 
-locale SimulateTransitive =
-  sim1: Simulate asrc adst aevt ainit atrans msrc mdst mevt minit mtrans r1
-+ sim2: Simulate msrc mdst mevt minit mtrans csrc cdst cevt cinit ctrans r2
+locale SimulateCompose =
+  sim1: Simulate la lb + sim2: Simulate lb lc
 for
-  asrc :: "'atrans \<Rightarrow> 'astate" and
-  adst :: "'atrans \<Rightarrow> 'astate" and
-  aevt :: "'atrans \<Rightarrow> 'event" and
-  ainit :: "'astate set" and
-  atrans :: "'atrans set" and
-  msrc :: "'mtrans \<Rightarrow> 'mstate" and
-  mdst :: "'mtrans \<Rightarrow> 'mstate" and
-  mevt :: "'mtrans \<Rightarrow> 'event" and
-  minit :: "'mstate set" and
-  mtrans :: "'mtrans set" and
-  r1 :: "('astate \<times> 'mstate) set" and
-  csrc :: "'ctrans \<Rightarrow> 'cstate" and
-  cdst :: "'ctrans \<Rightarrow> 'cstate" and
-  cevt :: "'ctrans \<Rightarrow> 'event" and
-  cinit :: "'cstate set" and
-  ctrans :: "'ctrans set" and
-  r2 :: "('mstate \<times> 'cstate) set"
+  la :: "('a, 'ev) LTS" and lb :: "('b, 'ev) LTS" and
+  lc :: "('c, 'ev) LTS"
+begin
+end
 
-sublocale SimulateTransitive \<subseteq> 
-          SimulationComposition
-                   asrc adst aevt ainit atrans msrc mdst mevt minit mtrans r1
-                   csrc cdst cevt cinit ctrans r2
-by unfold_locales
-
-sublocale SimulateTransitive \<subseteq> 
-          Simulate asrc adst aevt ainit atrans
-                   csrc cdst cevt cinit ctrans
-                   "r1 O r2"
-by unfold_locales
+sublocale SimulateCompose \<subseteq> Simulate la lc
+sorry
 
 end
